src/impl/TLS13.Impl.Server.Driver.Local.fsti
@@ -45,7 +45,7 @@ fn start_server_once
             'sent
 
 noextract
-val server_driver_local_write_correct
+let server_driver_local_write_correct
   (st0:CS.connection_state)
   (st1:CS.connection_state)
   (resp:ST.server_response)
@@ -53,7 +53,19 @@ val server_driver_local_write_correct
   (payload:B.bytes)
   (sent:B.bytes)
   (sent':B.bytes)
-  : prop
+  : prop =
+  exists network_out_bytes app_out_bytes.
+    ST.server_local_event_end_to_end_correct
+      st0
+      st1
+      resp
+      kind
+      payload
+      network_out_bytes
+      app_out_bytes /\
+    Seq.equal
+      sent'
+      (B.append sent (ST.response_network_out resp network_out_bytes))
 
 val lemma_server_driver_local_write_correct_intro
   (st0:CS.connection_state)
